Lib/Encode_Nat/Lifting_Nat.thy
@@ -11,30 +11,30 @@ unbundle lifting_syntax
 
 (* TODO: still necessary? *)
 lemma Domainp_nat_bool_rel[transfer_domain_rule]:
-  "Domainp (cr_nat :: _ \<Rightarrow> bool \<Rightarrow> _) = (\<lambda>x. x = False_nat \<or> x = True_nat)"
-  unfolding cr_nat_def Abs_nat_bool.simps
+  "Domainp (Rel_nat :: _ \<Rightarrow> bool \<Rightarrow> _) = (\<lambda>x. x = False_nat \<or> x = True_nat)"
+  unfolding Rel_nat_def natify_bool.simps
   by (auto split:bool.split)
 
 (* TODO: still necessary? *)
 lemma nat_bool_rel_conj[transfer_rule]:
-  "(cr_nat ===> cr_nat ===> cr_nat) max (\<and>)"
-  unfolding cr_nat_def Abs_nat_bool.simps
+  "(Rel_nat ===> Rel_nat ===> Rel_nat) max (\<and>)"
+  unfolding Rel_nat_def natify_bool.simps
   by (simp add: pair_def True_nat_def prod_encode_0 rel_fun_def split: bool.split)
 
 (* TODO: still necessary? *)
 lemma nat_bool_rel_disj[transfer_rule]:
-  "(cr_nat ===> cr_nat ===> cr_nat) min (\<or>)"
-  unfolding cr_nat_def Abs_nat_bool.simps
+  "(Rel_nat ===> Rel_nat ===> Rel_nat) min (\<or>)"
+  unfolding Rel_nat_def natify_bool.simps
   by (simp add: pair_def True_nat_def prod_encode_0 rel_fun_def split: bool.split)
 
 (* Example? *)
 schematic_goal
-  shows "cr_nat ?t (a \<and> (b \<or> c))"
+  shows "Rel_nat ?t (a \<and> (b \<or> c))"
   by transfer_prover
 
 
 
-(* lift_nat *)
+(* compile_nat *)
 
 
 
@@ -45,86 +45,87 @@ fun elemof :: "'a \<Rightarrow> 'a list \<Rightarrow> bool" where
 | "elemof y (x#xs) = (if (y = x) then True else elemof y xs)"
 
 
-function_lift_nat elemof
+function_compile_nat elemof
 
 (*
 lemma elemof_related_self [trp_in_dom]:
-  "(lift_nat_type_def.R \<Rrightarrow> lift_nat_type_def.R \<Rrightarrow> lift_nat_type_def.R) elemof elemof"
+  "(compile_nat_type_def.R \<Rrightarrow> compile_nat_type_def.R \<Rrightarrow> compile_nat_type_def.R) elemof elemof"
   unfolding Fun_Rel_rel_def
   by auto
 
-trp_term elemof_nat :: "nat \<Rightarrow> nat \<Rightarrow> nat" where x = "elemof :: ('a :: lift_nat) \<Rightarrow> _"
+trp_term elemof_nat :: "nat \<Rightarrow> nat \<Rightarrow> nat" where x = "elemof :: ('a :: compile_nat) \<Rightarrow> _"
   by trp_prover
 
 lemma elemof_nat_lifting[transfer_rule]:
-  shows "(cr_nat ===> cr_nat ===> cr_nat) (elemof_nat TYPE('a::lift_nat)) (elemof :: 'a \<Rightarrow> _)"
+  shows "(Rel_nat ===> Rel_nat ===> Rel_nat) (elemof_nat TYPE('a::compile_nat)) (elemof :: 'a \<Rightarrow> _)"
   unfolding rel_fun_eq_Fun_Rel_rel
   by (fact elemof_nat_related'[unfolded rel_inv_Fun_Rel_rel_eq[symmetric] rel_inv_iff_rel])
 
 schematic_goal elemof_nat_synth:
-  assumes [transfer_rule]: "(cr_nat :: nat \<Rightarrow> 'a \<Rightarrow> bool) xn (Rep_nat xn)"
-  assumes [transfer_rule]: "(cr_nat :: nat \<Rightarrow> 'a list \<Rightarrow> bool) xsn (Rep_nat xsn)"
-  shows "cr_nat ?t ((elemof :: 'a::lift_nat \<Rightarrow> _) (Rep_nat xn) (Rep_nat xsn))"
+  assumes [transfer_rule]: "(Rel_nat :: nat \<Rightarrow> 'a \<Rightarrow> bool) xn (denatify xn)"
+  assumes [transfer_rule]: "(Rel_nat :: nat \<Rightarrow> 'a list \<Rightarrow> bool) xsn (denatify xsn)"
+  shows "Rel_nat ?t ((elemof :: 'a::compile_nat \<Rightarrow> _) (denatify xn) (denatify xsn))"
   apply (subst elemof_case_def)
   by transfer_prover
  *)
 
 (* lemma elemof_nat_synth_def:
-  fixes x :: "'a::lift_nat " and xs :: "'a list"
-  assumes "xn = Abs_nat x"
-  assumes "xsn = Abs_nat xs"
+  fixes x :: "'a::compile_nat " and xs :: "'a list"
+  assumes "xn = natify_x"
+  assumes "xsn = natify_xs"
   shows "elemof_nat TYPE('a) xn xsn
     = case_list_nat False_nat (\<lambda>y ys. if xn = y then True_nat else elemof_nat TYPE('a) xn ys) xsn"
-  apply(rule HOL.trans[OF _ elemof_nat_synth[unfolded cr_nat_def, symmetric]])
-    apply(simp add: elemof_nat_app_eq assms; subst Rep_nat_Abs_nat_id)+
+  apply(rule HOL.trans[OF _ elemof_nat_synth[unfolded Rel_nat_def, symmetric]])
+    apply(simp add: elemof_nat_app_eq assms; subst denatify_natify_id)+
   done *)
 
 thm elemof_nat_synth_def[unfolded case_list_nat_def]
-
 
 fun takeWhile :: "('a \<Rightarrow> bool) \<Rightarrow> 'a list \<Rightarrow> 'a list" where
   "takeWhile P [] = []" |
   "takeWhile P (x # xs) = (if P x then x # takeWhile P xs else [])"
 
-(* TODO: Not working yet :( something in mk_trp_term *)
-function_lift_nat takeWhile
+(* TODO: goals for higher-order set up the wrong way*)
+(* Note Kevin: do you really want "Rel_nat ni (denatify ni)" as assumptions?
+  Why not the more general theorem with assumptions "Rel_nat ni xi" ? *)
+function_compile_nat takeWhile
 
 case_of_simps takeWhile_case_def: takeWhile.simps
 
 unbundle no_comp_syntax
 
 lemma takeWhile_related_self [trp_in_dom]:
-  "((lift_nat_type_def.R \<Rrightarrow> lift_nat_type_def.R) \<Rrightarrow> lift_nat_type_def.R \<Rrightarrow> lift_nat_type_def.R)
+  "((compile_nat_type_def.R \<Rrightarrow> compile_nat_type_def.R) \<Rrightarrow> compile_nat_type_def.R \<Rrightarrow> compile_nat_type_def.R)
   takeWhile takeWhile"
   by auto
 
 trp_term takeWhile_nat :: "(nat \<Rightarrow> nat) \<Rightarrow> nat \<Rightarrow> nat"
-  where x = "takeWhile :: (('a :: lift_nat) \<Rightarrow> bool) \<Rightarrow> _"
+  where x = "takeWhile :: (('a :: compile_nat) \<Rightarrow> bool) \<Rightarrow> _"
   by trp_prover
 
 lemma takeWhile_nat_lifting[transfer_rule]:
-  "((cr_nat ===> cr_nat) ===> cr_nat ===> cr_nat)
-  (takeWhile_nat TYPE('a::lift_nat)) ((takeWhile :: ('a \<Rightarrow> bool) \<Rightarrow> _))"
+  "((Rel_nat ===> Rel_nat) ===> Rel_nat ===> Rel_nat)
+  (takeWhile_nat TYPE('a::compile_nat)) ((takeWhile :: ('a \<Rightarrow> bool) \<Rightarrow> _))"
   using takeWhile_nat_related'
   by(simp add: takeWhile_nat_related' rel_fun_eq_Fun_Rel_rel flip: rel_inv_Fun_Rel_rel_eq)
 
 
 schematic_goal takeWhile_nat_synth:
-  assumes [transfer_rule]: "(cr_nat :: nat \<Rightarrow> 'a list \<Rightarrow> bool) xsn (Rep_nat xsn)"
-  assumes [transfer_rule]: "(cr_nat ===> cr_nat) P_nat P"
-  shows "cr_nat ?t ((takeWhile :: ('a::lift_nat \<Rightarrow> bool) \<Rightarrow> _) P (Rep_nat xsn))"
+  assumes [transfer_rule]: "(Rel_nat :: nat \<Rightarrow> 'a list \<Rightarrow> bool) xsn (denatify xsn)"
+  assumes [transfer_rule]: "(Rel_nat ===> Rel_nat) P_nat P"
+  shows "Rel_nat ?t ((takeWhile :: ('a::compile_nat \<Rightarrow> bool) \<Rightarrow> _) P (denatify xsn))"
   by (subst takeWhile_case_def) transfer_prover
 
 lemma takeWhile_nat_synth_def:
-  fixes P :: "'a::lift_nat \<Rightarrow> bool" and xs :: "'a list"
-  assumes "(cr_nat ===> cr_nat) P_nat P"
-  assumes "xsn = Abs_nat xs"
+  fixes P :: "'a::compile_nat \<Rightarrow> bool" and xs :: "'a list"
+  assumes "(Rel_nat ===> Rel_nat) P_nat P"
+  assumes "xsn = natify_xs"
   shows "takeWhile_nat TYPE('a) P_nat xsn
     = case_list_nat Nil_nat (\<lambda>x3a x2ba. If_nat TYPE('a list) (P_nat x3a)
           (Cons_nat x3a (takeWhile_nat TYPE('a) P_nat x2ba)) Nil_nat) xsn"
-  apply(rule HOL.trans[OF _ takeWhile_nat_synth[unfolded cr_nat_def, symmetric]])
+  apply(rule HOL.trans[OF _ takeWhile_nat_synth[unfolded Rel_nat_def, symmetric]])
   using assms
-    apply(simp add: assms takeWhile_nat_app_eq rel_fun_def cr_nat_def)+
+    apply(simp add: assms takeWhile_nat_app_eq rel_fun_def Rel_nat_def)+
   done
 
 thm takeWhile_nat_synth_def[unfolded case_list_nat_def]
@@ -133,31 +134,31 @@ fun head :: "'a list \<Rightarrow> 'a" where
   "head [] = undefined" |
   "head (x # _) = x"
 
-function_lift_nat head
+function_compile_nat head
   (*
 case_of_simps head_case_def: head.simps
 
-definition head_nat :: "'a::lift_nat itself \<Rightarrow> nat \<Rightarrow> nat" where
-  "head_nat _ xsn \<equiv> (Abs_nat :: 'a \<Rightarrow> nat) (head (Rep_nat xsn))"
+definition head_nat :: "'a::compile_nat itself \<Rightarrow> nat \<Rightarrow> nat" where
+  "head_nat _ xsn \<equiv> (natify_:: 'a \<Rightarrow> nat) (head (denatify xsn))"
 
 lemma head_nat_lifting[transfer_rule]:
-  shows "(cr_nat ===> cr_nat) (head_nat TYPE('a::lift_nat)) (head :: 'a list \<Rightarrow> _)"
-  unfolding head_nat_def cr_nat_def
+  shows "(Rel_nat ===> Rel_nat) (head_nat TYPE('a::compile_nat)) (head :: 'a list \<Rightarrow> _)"
+  unfolding head_nat_def Rel_nat_def
   by(simp add: rel_fun_def)
 
 schematic_goal head_nat_synth:
-  assumes [transfer_rule]: "(cr_nat :: nat \<Rightarrow> 'a list \<Rightarrow> bool) xsn (Rep_nat xsn)"
-  shows "cr_nat ?t ((head :: 'a::lift_nat list \<Rightarrow> _) (Rep_nat xsn))"
+  assumes [transfer_rule]: "(Rel_nat :: nat \<Rightarrow> 'a list \<Rightarrow> bool) xsn (denatify xsn)"
+  shows "Rel_nat ?t ((head :: 'a::compile_nat list \<Rightarrow> _) (denatify xsn))"
   apply (subst head_case_def)
   by transfer_prover *)
 
 (* lemma head_nat_synth_def:
-  fixes xs :: "'a::lift_nat list"
-  assumes "xsn = Abs_nat xs"
+  fixes xs :: "'a::compile_nat list"
+  assumes "xsn = natify_xs"
   shows "head_nat TYPE('a) xsn
-    = case_list_nat (Abs_nat (undefined::'a)) (\<lambda>x2a x1a. x2a) xsn"
-  apply(rule HOL.trans[OF _ head_nat_synth[unfolded cr_nat_def, symmetric]])
-   apply(simp add: head_nat_app_eq assms; subst Rep_nat_Abs_nat_id)+
+    = case_list_nat (natify_(undefined::'a)) (\<lambda>x2a x1a. x2a) xsn"
+  apply(rule HOL.trans[OF _ head_nat_synth[unfolded Rel_nat_def, symmetric]])
+   apply(simp add: head_nat_app_eq assms; subst denatify_natify_id)+
   done *)
 
 thm head_nat_synth_def[unfolded case_list_nat_def]
@@ -166,33 +167,33 @@ fun append :: "'a list \<Rightarrow> 'a list \<Rightarrow> 'a list" where
   "append xs [] = xs" |
   "append xs ys = rev_tr ys (rev_tr [] xs)"
 
-function_lift_nat append
+function_compile_nat append
 
 (* case_of_simps append_case_def: append.simps
 
-definition append_nat :: "'a::lift_nat itself \<Rightarrow> nat \<Rightarrow> nat \<Rightarrow> nat" where
-  "append_nat _ xsn ysn \<equiv> (Abs_nat :: 'a list \<Rightarrow> nat) (append (Rep_nat xsn) (Rep_nat ysn))"
+definition append_nat :: "'a::compile_nat itself \<Rightarrow> nat \<Rightarrow> nat \<Rightarrow> nat" where
+  "append_nat _ xsn ysn \<equiv> (natify_:: 'a list \<Rightarrow> nat) (append (denatify xsn) (denatify ysn))"
 
 lemma append_nat_lifting[transfer_rule]:
-  shows "(cr_nat ===> cr_nat ===> cr_nat) (append_nat TYPE('a::lift_nat))
+  shows "(Rel_nat ===> Rel_nat ===> Rel_nat) (append_nat TYPE('a::compile_nat))
   (append :: 'a list \<Rightarrow> 'a list \<Rightarrow> 'a list)"
-  by(simp add: append_nat_def rel_fun_def Fun.comp_def cr_nat_def)
+  by(simp add: append_nat_def rel_fun_def Fun.comp_def Rel_nat_def)
 
 schematic_goal append_nat_synth:
-  assumes [transfer_rule]: "(cr_nat :: nat \<Rightarrow> 'a list \<Rightarrow> bool) xsn (Rep_nat xsn)"
-  assumes [transfer_rule]: "(cr_nat :: nat \<Rightarrow> 'a list \<Rightarrow> bool) ysn (Rep_nat ysn)"
-  shows "cr_nat ?t ((append :: 'a::lift_nat list \<Rightarrow> _) (Rep_nat xsn) (Rep_nat ysn))"
+  assumes [transfer_rule]: "(Rel_nat :: nat \<Rightarrow> 'a list \<Rightarrow> bool) xsn (denatify xsn)"
+  assumes [transfer_rule]: "(Rel_nat :: nat \<Rightarrow> 'a list \<Rightarrow> bool) ysn (denatify ysn)"
+  shows "Rel_nat ?t ((append :: 'a::compile_nat list \<Rightarrow> _) (denatify xsn) (denatify ysn))"
   apply (subst append_case_def)
   by transfer_prover *)
 
 (* lemma append_nat_synth_def:
-  fixes xs :: "'a::lift_nat list" and ys :: "'a list"
-  assumes "xsn = Abs_nat xs"
-  assumes "ysn = Abs_nat ys"
+  fixes xs :: "'a::compile_nat list" and ys :: "'a list"
+  assumes "xsn = natify_xs"
+  assumes "ysn = natify_ys"
   shows "append_nat TYPE('a) xsn ysn = case_list_nat xsn (\<lambda>x3a x2ba. rev_tr_nat TYPE('a)
                 (Cons_nat x3a x2ba) (rev_tr_nat TYPE('a) Nil_nat xsn)) ysn"
-  apply(rule HOL.trans[OF _ append_nat_synth[unfolded cr_nat_def, symmetric]])
-    apply(simp add: append_nat_app_eq assms; subst Rep_nat_Abs_nat_id)+
+  apply(rule HOL.trans[OF _ append_nat_synth[unfolded Rel_nat_def, symmetric]])
+    apply(simp add: append_nat_app_eq assms; subst denatify_natify_id)+
   done
  *)
 
@@ -203,13 +204,13 @@ fun plus :: "nat \<Rightarrow> nat \<Rightarrow> nat" where
 
 
 (* TODO: Not working yet :( something in mk_trp_term *)
-function_lift_nat plus
+function_compile_nat plus
 
 case_of_simps plus_case_def: plus.simps
 
 
 lemma plus_related_self [trp_in_dom]:
-  "(lift_nat_type_def.R \<Rrightarrow> lift_nat_type_def.R \<Rrightarrow> lift_nat_type_def.R) plus plus"
+  "(compile_nat_type_def.R \<Rrightarrow> compile_nat_type_def.R \<Rrightarrow> compile_nat_type_def.R) plus plus"
   unfolding Fun_Rel_rel_def
   by auto
 
@@ -218,25 +219,25 @@ trp_term plus_nat :: "nat \<Rightarrow> nat \<Rightarrow> nat" where x = "plus"
 
 
 lemma plus_nat_lifting[transfer_rule]:
-  shows "(cr_nat ===> cr_nat ===> cr_nat) plus_nat plus"
-  using plus_nat_app_eq by(simp add: rel_fun_def cr_nat_def)
+  shows "(Rel_nat ===> Rel_nat ===> Rel_nat) plus_nat plus"
+  using plus_nat_app_eq by(simp add: rel_fun_def Rel_nat_def)
 
 schematic_goal plus_nat_synth:
-  assumes [transfer_rule]: "(cr_nat :: nat \<Rightarrow> nat \<Rightarrow> bool) mn (Rep_nat mn)"
-  assumes [transfer_rule]: "(cr_nat :: nat \<Rightarrow> nat \<Rightarrow> bool) nn (Rep_nat nn)"
-  shows "cr_nat ?t (plus (Rep_nat mn) (Rep_nat nn))"
+  assumes [transfer_rule]: "(Rel_nat :: nat \<Rightarrow> nat \<Rightarrow> bool) mn (denatify mn)"
+  assumes [transfer_rule]: "(Rel_nat :: nat \<Rightarrow> nat \<Rightarrow> bool) nn (denatify nn)"
+  shows "Rel_nat ?t (plus (denatify mn) (denatify nn))"
   apply (subst plus_case_def)
   by transfer_prover
 
 lemma plus_nat_synth_def:
   fixes m :: nat and n :: nat
-  assumes "mn = Abs_nat m"
-  assumes "nn = Abs_nat n"
+  assumes "mn = natify_m"
+  assumes "nn = natify_n"
   shows "plus_nat mn nn
     = case_nat_nat mn (\<lambda>x2ba. Suc_nat (plus_nat mn x2ba)) nn"
-  apply(rule HOL.trans[OF _ plus_nat_synth[unfolded cr_nat_def, symmetric]])
+  apply(rule HOL.trans[OF _ plus_nat_synth[unfolded Rel_nat_def, symmetric]])
   using assms
-    apply(simp add: plus_nat_app_eq; subst Rep_nat_Abs_nat_id)+
+    apply(simp add: plus_nat_app_eq; subst denatify_natify_id)+
   done
 
 thm plus_nat_synth_def[unfolded case_nat_nat_def]
